@prefix rdf: <http://www.w3.org/1999/02/22-rdf-syntax-ns#> .
@prefix rdfs: <http://www.w3.org/2000/01/rdf-schema#> .
@prefix owl: <http://www.w3.org/2002/07/owl#> .
@prefix vann: <http://purl.org/vocab/vann/> .
@prefix dcterms: <http://purl.org/dc/terms/> .
@prefix xsd: <http://www.w3.org/2001/XMLSchema#> .
@prefix foaf: <http://xmlns.com/foaf/0.1/> .
@prefix fairnet: <http://localhost:8443/public/voc/fairnet.ttl#> .

fairnet: rdf:type owl:Ontology ;
    # Descriptiona
    dcterms:title "Post ontology" ;
    dcterms:description """
    The fairnet ontology aims at describing fairnet and post.
    """ ;
    vann:preferredNamespacePrefix "fairnet" ;
    vann:preferredNamespaceURI <http://localhost:8443/public/voc/fairnet.ttl#> ;
    # Ownership
    dcterms:license <http://creativecommons.org/licenses/by/4.0/> ;
    dcterms:creator <https://localhost:8443/profile/card#me> ;
    dcterms:contributor <https://localhost:8443/profile/card#me> ;
    # dcterms:publisher <https://jcaesar.solid.community/profile/organizations/spqr.ttl#spqr>;
    # Version
    # owl:versionIRI <http://localhost:8443/public/voc/fairnet/2019/10/09/ns> ;
    # owl:priorVersion <http://localhost:8443/public/voc/fairnet/2019/10/08/ns> ;
    # dcterms:isReplacedBy <http://localhost:8443/public/voc/fairnet/2019/10/08/ns> ;
    owl:versionInfo "0.1.0" ;
    dcterms:issued "2021-10-09" ;
    dcterms:modified "2021-10-09".

fairnet:Post a rdfs:Class ;
    rdfs:label "Post"@en ;
    rdfs:comment "A post is something that its creator posted on a social network service."@en .

fairnet:ownedBy a owl:ObjectProperty ;
    rdfs:label "owned by"@en ;
    rdfs:comment "Relationship between a post and the person who created and posted it."@en ;
    rdfs:domain fairnet:Post ;
    rdfs:range foaf:Person .

fairnet:title a owl:DatatypeProperty ;
    rdfs:label "title"@en ;
    rdfs:comment "The title of the post."@en ;
    rdfs:domain fairnet:Post ;
    rdfs:range xsd:string.

fairnet:content a owl:DatatypeProperty ;
    rdfs:label "content"@en ;
    rdfs:comment "The content of the post."@en ;
    rdfs:domain fairnet:Post ;
    rdfs:range xsd:string.

